---
tags:
  - Physics/Fields/Gravitational
---
# Satellite Motion
A Satellite can refer to any object orbiting another object. From the human made satellites (which the word is more commonly associated with) to natural satellites, such as the Earth's moon & the two moons orbiting Mars (Phobos & Deimos).

`Using formula from Circular motion because satellite orbits are being modelled as a circle?`
Newton realised that the [[Physics/Further Mechanics/Circular motion/Centripetal Force|Centripetal Force]] that keeps each planet on its orbit is equal to the force of gravitational attraction between the planet & the sun.
[[Physics/Further Mechanics/Circular motion/Centripetal Force|Centripetal Force]] can be derived from "$\frac{mv^2}{r}$".
The gravitational force can be derived from "$\frac{GMm}{r^2}$"
Since both of the above derivations are equal to *Force* they can be used to find the velocity of a planet (a satellite of the sun).
$=> \frac{mv^2}{r} = \frac{GMm}{r^2}$
$=> \frac{v^2}{r} = \frac{GM}{r^2}$
$=> v^2 = \frac{GM}{r}$
$=> v = \sqrt{\frac{GM}{r}} = \sqrt{GMr^{-1}}$
Where:
$v$ = The velocity of the satellite
$G$ = Gravitational constant
$M$ = Mass of the orbited object
$r$ = Mean radius of the orbit
(This equation is not in the data sheet)

Further work with this formula can be used to prove that [[Physics/Fields/Gravitational/Kepler's Third Law|Kepler's Third Law]] as true. The resulting formula for this proof is "$\frac{r^3}{T^2} = \frac{GM}{4\pi^2}$" where:
$r$ = The mean radius of the orbit
$T$ = The time period of the orbit
$G$ = Gravitational constant
$M$ = Mass of the orbited Object

// Keep?
Furthermore, it can be shown that "$v$" has a relationship to time by:
$\omega = \frac{v}{r}$
$=> v = \omega r$
Then,
$\omega = 2\pi f$
$f = \frac{1}{T}$
$=> \omega = \frac{2\pi}{T}$
Then substituting it to get,
$v = \frac{2\pi r}{T}$
// Keep?

## Satellite Energy
The total energy of a satellite in orbit is always negative as gravity is an **attractive** force. The total energy of a satellite can be calculated by summing the [[Physics/Kinetic Energy|Kinetic Energy]] & [[Physics/Fields/Gravitational/Gravitational Potential|Gravitational Potential]] together. The combined formula for this is "$E = -\frac{GMm}{2r}$" with:
$E$ = Energy of the satellite
$G$ = Gravitational constant
$M$ = Mass of the orbited object
$m$ = Mass of the orbiting object
$r$ = Mean radius of the orbit